DynamoDbEncryption/dafny/StructuredEncryption/src/Crypt.dfy
@@ -127,14 +127,45 @@ module StructuredEncryptionCrypt {
 
   datatype EncryptionSelector = DoEncrypt | DoDecrypt
 
-  predicate Updated(oldVal : CanonCryptoItem, newVal : CanonCryptoItem)
+  predicate Updated(oldVal : CanonCryptoItem, newVal : CanonCryptoItem, mode : EncryptionSelector)
   {
     && oldVal.key == newVal.key
     && oldVal.origKey == newVal.origKey
     && oldVal.action == newVal.action
-    && (oldVal.action != ENCRYPT_AND_SIGN <==> oldVal.data == newVal.data)
-    && (oldVal.action == ENCRYPT_AND_SIGN <==> oldVal.data != newVal.data)
+    && (newVal.action != ENCRYPT_AND_SIGN <==> oldVal.data == newVal.data)
+    && (newVal.action == ENCRYPT_AND_SIGN <==> oldVal.data != newVal.data)
+    && (mode == DoEncrypt ==> (newVal.action == ENCRYPT_AND_SIGN ==> newVal.data.typeId == BYTES_TYPE_ID))
+    && (mode == DoDecrypt ==> (newVal.action == ENCRYPT_AND_SIGN ==> |oldVal.data.value| >= 2 && newVal.data.typeId == oldVal.data.value[..2]))
   }
+
+  predicate Updated2(oldVal : AuthItem, newVal : CanonCryptoItem, mode : EncryptionSelector)
+  {
+    && oldVal.key == newVal.origKey
+    && (newVal.action != ENCRYPT_AND_SIGN <==> oldVal.data == newVal.data)
+    && (newVal.action == ENCRYPT_AND_SIGN <==> oldVal.data != newVal.data)
+    && (mode == DoEncrypt ==> (newVal.action == ENCRYPT_AND_SIGN ==> newVal.data.typeId == BYTES_TYPE_ID))
+    && (mode == DoDecrypt ==> (newVal.action == ENCRYPT_AND_SIGN ==> |oldVal.data.value| >= 2 && newVal.data.typeId == oldVal.data.value[..2]))
+  }
+
+  predicate Updated3(oldVal : AuthItem, newVal : CryptoItem, mode : EncryptionSelector)
+  {
+    && oldVal.key == newVal.key
+    && (newVal.action != ENCRYPT_AND_SIGN <==> oldVal.data == newVal.data)
+    && (newVal.action == ENCRYPT_AND_SIGN <==> oldVal.data != newVal.data)
+    && (mode == DoEncrypt ==> (newVal.action == ENCRYPT_AND_SIGN ==> newVal.data.typeId == BYTES_TYPE_ID))
+    && (mode == DoDecrypt ==> (newVal.action == ENCRYPT_AND_SIGN ==> |oldVal.data.value| >= 2 && newVal.data.typeId == oldVal.data.value[..2]))
+  }
+
+  predicate Updated4(oldVal : CryptoItem, newVal : CryptoItem, mode : EncryptionSelector)
+  {
+    && oldVal.key == newVal.key
+    && oldVal.action == newVal.action
+    && (newVal.action != ENCRYPT_AND_SIGN <==> oldVal.data == newVal.data)
+    && (newVal.action == ENCRYPT_AND_SIGN <==> oldVal.data != newVal.data)
+    && (mode == DoEncrypt ==> (newVal.action == ENCRYPT_AND_SIGN ==> newVal.data.typeId == BYTES_TYPE_ID))
+    && (mode == DoDecrypt ==> (newVal.action == ENCRYPT_AND_SIGN ==> |oldVal.data.value| >= 2 && newVal.data.typeId == oldVal.data.value[..2]))
+  }
+
 
   // Encrypt a StructuredDataMap
   method Encrypt(
@@ -151,8 +182,7 @@ module StructuredEncryptionCrypt {
     ensures client.ValidState()
     ensures ret.Success? ==>
               && |ret.value| == |data|
-              && (forall i | 0 <= i < |data| :: Updated(data[i], ret.value[i]))
-              && (forall x | 0 <= x < |ret.value| :: (ret.value[x].action == ENCRYPT_AND_SIGN ==> ret.value[x].data.typeId == BYTES_TYPE_ID))
+              && (forall i | 0 <= i < |data| :: Updated(data[i], ret.value[i], DoEncrypt))
   {
     ret := Crypt(DoEncrypt, client, alg, key, head, data);
   }
@@ -172,7 +202,7 @@ module StructuredEncryptionCrypt {
     ensures client.ValidState()
     ensures ret.Success? ==>
               && |ret.value| == |data|
-              && forall i | 0 <= i < |data| :: Updated(data[i], ret.value[i])
+              && forall i | 0 <= i < |data| :: Updated(data[i], ret.value[i], DoDecrypt)
   {
     ret := Crypt(DoDecrypt, client, alg, key, head, data);
   }
@@ -221,8 +251,7 @@ module StructuredEncryptionCrypt {
     ensures client.ValidState()
     ensures ret.Success? ==>
               && |ret.value| == |data|
-              && (forall i | 0 <= i < |data| :: Updated(data[i], ret.value[i]))
-              && ((mode == DoEncrypt) ==> forall x | 0 <= x < |ret.value| :: (ret.value[x].action == ENCRYPT_AND_SIGN ==> ret.value[x].data.typeId == BYTES_TYPE_ID))
+              && (forall i | 0 <= i < |data| :: Updated(data[i], ret.value[i], mode))
   {
     //= specification/structured-encryption/encrypt-path-structure.md#calculate-cipherkey-and-nonce
     //# The `FieldRootKey` MUST be generated with the plaintext data key in the encryption materials
@@ -262,8 +291,7 @@ module StructuredEncryptionCrypt {
     ensures client.ValidState()
     ensures ret.Success? ==>
               && |ret.value| == |data|
-              && (forall i | 0 <= i < |data| :: Updated(data[i], ret.value[i]))
-              && ((mode == DoEncrypt) ==> forall x | 0 <= x < |ret.value| :: (ret.value[x].action == ENCRYPT_AND_SIGN ==> ret.value[x].data.typeId == BYTES_TYPE_ID))
+              && (forall i | 0 <= i < |data| :: Updated(data[i], ret.value[i], mode))
   {
     var result : CanonCryptoList := [];
     var pos : uint32 := 0;
@@ -271,8 +299,7 @@ module StructuredEncryptionCrypt {
     for i := 0 to |data|
       invariant pos <= (i as uint32)
       invariant |result| == i
-      invariant forall x | 0 <= x < |result| :: Updated(data[x], result[x])
-      invariant (mode == DoEncrypt) ==> forall x | 0 <= x < |result| :: (result[x].action == ENCRYPT_AND_SIGN ==> result[x].data.typeId == BYTES_TYPE_ID)
+      invariant forall x | 0 <= x < |result| :: Updated(data[x], result[x], mode)
     {
       if data[i].action == ENCRYPT_AND_SIGN {
         var newTerminal;
@@ -285,12 +312,12 @@ module StructuredEncryptionCrypt {
         pos := pos + 1;
         var newItem := data[i].(data := newTerminal);
         result := result + [newItem];
-        assert Updated(data[i], result[i]);
+        assert Updated(data[i], result[i], mode);
       } else {
         result := result + [data[i]];
-        assert Updated(data[i], result[i]);
+        assert Updated(data[i], result[i], mode);
       }
-      assert Updated(data[i], result[i]);
+      assert Updated(data[i], result[i], mode);
     }
     return Success(result);
   }
